theories/Handlers/Deterministic.v
@@ -1,0 +1,138 @@
+(* SLOT, a formally verified model checker
+   Copyright (C) 2019-2021  k32
+
+   This program is free software: you can redistribute it and/or modify
+   it under the terms of the GNU General Public License as published by
+   the Free Software Foundation, version 3 of the License.
+
+   This program is distributed in the hope that it will be useful,
+   but WITHOUT ANY WARRANTY; without even the implied warranty of
+   MERCHANTABILITY or FITNESS FOR A PARTICULAR PURPOSE.  See the
+   GNU General Public License for more details.
+
+   You should have received a copy of the GNU General Public License
+   along with this program.  If not, see <https://www.gnu.org/licenses/>.
+*)
+
+(** * Generic total deterministic IO handler *)
+From Coq Require Import
+     List.
+
+From stdpp Require Import
+     fin_maps.
+
+From SLOT Require Import
+     Foundations.
+
+Class DeterministicHandler (Req : Type) (Ret : Req -> Type) :=
+  { det_h_state : Type;
+    det_h_state_transition : forall (pid : PID) (s : det_h_state) (req : Req), det_h_state * Ret req;
+  }.
+
+Global Instance deterministicHandler `{d : DeterministicHandler} : @IOHandler Req Ret :=
+  { h_state_transition s te s' :=
+      match te with
+      | proc_te pid (iop req ret) =>
+        let (s'_, ret_) := det_h_state_transition pid s req in
+        s' = s'_ /\ ret = ret_
+      end;
+  }.
+
+Global Arguments deterministicHandler {_} {_}.
+
+Module Var.
+  Section defs.
+    Context {T : Type}.
+
+    Inductive var_req_t :=
+    | read
+    | write : T -> var_req_t.
+
+    Definition var_ret_t req :=
+      match req with
+      | read => T
+      | write _ => True
+      end.
+
+    Definition var_step (_ : PID) s req : T * var_ret_t req :=
+      match req with
+      | read => (s, s)
+      | write new => (new, I)
+      end.
+
+    Global Instance varDetHandler : DeterministicHandler var_req_t var_ret_t :=
+      { det_h_state := T;
+        det_h_state_transition := var_step;
+      }.
+  End defs.
+
+  Definition t T := deterministicHandler (@varDetHandler T).
+End Var.
+
+Module Log.
+  Section defs.
+    Context {Event : Type}.
+
+    Definition State : Type := list Event.
+
+    Definition hist_req_t := PID -> Event.
+
+    Definition step (pid : PID) (s : State) (req : hist_req_t) := (req pid :: s, I).
+
+    Global Instance historyDetHandler : DeterministicHandler hist_req_t (fun _ => True) :=
+      { det_h_state := list Event;
+        det_h_state_transition := step;
+      }.
+  End defs.
+
+  Definition t Event := deterministicHandler (@historyDetHandler Event).
+End Log.
+
+Global Arguments Log.t : clear implicits.
+
+Module ProcessDictionary.
+  Section defs.
+    Context {Val : Type} `{FinMap PID Map}.
+
+    Inductive req_t : Type :=
+    | pd_get
+    | pd_erase
+    | pd_put : Val -> req_t.
+
+    Definition ret_t req : Type :=
+      match req with
+      | pd_get => option Val
+      | pd_put _ => True
+      | pd_erase => True
+      end.
+
+    Definition State := Map Val.
+
+    Definition step (pid : PID) (s : State) (req : req_t) : State * ret_t req :=
+      match req with
+      | pd_get => (s, s !! pid)
+      | pd_put new_val => (<[pid := new_val]> s, I)
+      | pd_erase => (delete pid s, I)
+      end.
+
+    Global Instance processDictDetHandler : DeterministicHandler req_t ret_t :=
+      { det_h_state := State;
+        det_h_state_transition := step;
+      }.
+
+    Definition t := deterministicHandler processDictDetHandler.
+  End defs.
+
+  Global Arguments t {_}.
+End ProcessDictionary.
+
+Module Self.
+  Inductive req_t := self.
+
+  Global Instance selfDetHandler : DeterministicHandler req_t (fun _ => PID) :=
+    { det_h_state := True;
+      det_h_state_transition pid _ _ := (I, pid)
+    }.
+
+  Definition t := deterministicHandler selfDetHandler.
+End Self.
