theories/Handlers/MQ.v
@@ -1,0 +1,90 @@
+(* SLOT, a formally verified model checker
+   Copyright (C) 2019-2021  k32
+
+   This program is free software: you can redistribute it and/or modify
+   it under the terms of the GNU General Public License as published by
+   the Free Software Foundation, version 3 of the License.
+
+   This program is distributed in the hope that it will be useful,
+   but WITHOUT ANY WARRANTY; without even the implied warranty of
+   MERCHANTABILITY or FITNESS FOR A PARTICULAR PURPOSE.  See the
+   GNU General Public License for more details.
+
+   You should have received a copy of the GNU General Public License
+   along with this program.  If not, see <https://www.gnu.org/licenses/>.
+*)
+
+(** * Distributed message queue
+
+    This IO handler implements a generic "message queue" service
+    similar to Apache Kafka. Every published message gets an integer
+    offset, and can later be fetched using the offset as a key.
+*)
+From Coq Require Import
+     List.
+
+Import ListNotations.
+
+
+From SLOT Require Import
+     Foundations.
+
+Section defs.
+  (** Parameters:
+      - [PID] type of process ids
+      - [T] type of message *)
+  Context {T : Type}.
+
+  Definition Offset := nat.
+
+  (** ** Syscalls:
+      This handler implements the following syscalls: *)
+
+  Inductive req_t :=
+  (** Nonblocking poll: *)
+  | poll : Offset -> req_t
+  (** Block execution of the caller until a message with the given
+  offset is produced by some other process: *)
+  | fetch : Offset -> req_t
+  (** Attempt to produce a message. This syscall is
+     nondeterministic, with the following possible outcomes:
+     - message gets successfully produced, and its offset is
+       returned to the caller as [Some Offset]
+     - message gets lost in transition, [None] is returned to the
+       caller
+     - message gets successfully produced, but the response gets
+       lost in transition. The caller gets [None] *)
+  | produce : T -> req_t.
+
+  Local Definition ret_t (req : req_t) : Type :=
+    match req with
+    | poll _ => option T
+    | fetch _ => T
+    | produce _ => option Offset
+    end.
+
+  Let TE := TraceElem req_t ret_t.
+  Let S := list T.
+
+  (** ** Possible state space transitions: *)
+  Inductive mq_state_transition : S -> TE -> S -> Prop :=
+  | mq_poll : forall s pid offset,
+      mq_state_transition s (pid @ nth_error s offset <~ poll offset) s
+  | mq_fetch : forall s pid offset val,
+      nth_error s offset = Some val ->
+      mq_state_transition s (pid @ val <~ fetch offset) s
+  (** Message is successfully produced: *)
+  | mq_produce : forall s pid val,
+      mq_state_transition s (pid @ Some (length s) <~ produce val) (val :: s)
+  (** Response is lost: *)
+  | mq_produce_lost_resp : forall s pid val,
+      mq_state_transition s (pid @ None <~ produce val) (val :: s)
+  (** Message is lost: *)
+  | mq_produce_lost_msg : forall s pid val,
+      mq_state_transition s (pid @ None <~ produce val) s.
+
+  Global Instance t : @IOHandler req_t ret_t :=
+    { h_state := S;
+      h_state_transition := mq_state_transition;
+    }.
+End defs.
