theories/Handlers/Mutex.v
@@ -1,0 +1,90 @@
+(* SLOT, a formally verified model checker
+   Copyright (C) 2019-2021  k32
+
+   This program is free software: you can redistribute it and/or modify
+   it under the terms of the GNU General Public License as published by
+   the Free Software Foundation, version 3 of the License.
+
+   This program is distributed in the hope that it will be useful,
+   but WITHOUT ANY WARRANTY; without even the implied warranty of
+   MERCHANTABILITY or FITNESS FOR A PARTICULAR PURPOSE.  See the
+   GNU General Public License for more details.
+
+   You should have received a copy of the GNU General Public License
+   along with this program.  If not, see <https://www.gnu.org/licenses/>.
+*)
+
+From Coq Require Import
+     List.
+
+Import ListNotations.
+
+From SLOT Require Import
+     Foundations
+     Properties
+     Tactics.
+
+Section defs.
+  Open Scope slot_scope.
+
+  Inductive req_t : Set :=
+  | grab    : req_t
+  | release : req_t.
+
+  Local Definition ret_t (req : req_t) : Set :=
+    match req with
+    | grab => True
+    | release => bool
+    end.
+
+  Definition state_t := option PID.
+
+  Let TE := TraceElem req_t ret_t.
+
+  Inductive mutex_state_transition : state_t -> TE -> state_t -> Prop :=
+  | mutex_grab : forall pid,
+      mutex_state_transition None (pid @ I <~ grab) (Some pid)
+  | mutex_release_ok : forall pid,
+      mutex_state_transition (Some pid) (pid @ true <~ release) None
+  | mutex_release_fail : forall pid,
+      mutex_state_transition None (pid @ false <~ release) None.
+
+  Global Instance mutexHandler : @IOHandler req_t ret_t :=
+    { h_state := state_t;
+      h_state_transition := mutex_state_transition;
+    }.
+
+  Theorem no_double_grab : forall (a1 a2 : PID),
+      {{ fun _  => True }}
+        [a1 @ I <~ grab;
+         a2 @ I <~ grab]
+      {{ fun _ => False }}.
+  Proof.
+    intros a1 a2 s s' Hss' Hpre.
+    unfold_trace_deep Hss'.
+    discriminate.
+  Qed.
+
+  Theorem no_double_grab_0 : forall (a1 a2 : PID),
+      ~(PossibleTrace [a1 @ I <~ grab;
+                       a2 @ I <~ grab]).
+  Proof.
+    intros a1 a2 H.
+    destruct H as [s [s' H]].
+    unfold_trace_deep H.
+    discriminate.
+  Qed.
+End defs.
+
+Ltac mutex_contradiction :=
+  match goal with
+    [H1 : mutex_state_transition _ ?s1 ?s2 _, H2 : mutex_state_transition _ ?s2 ?s3 _ |- _] =>
+      inversion H1; inversion H2; subst; discriminate
+  end.
+
+Hint Extern 4 => mutex_contradiction : handlers.
+
+Ltac clear_mutex :=
+  repeat match goal with
+           [H: mutex_state_transition _ _ _ _ |- _] => clear H
+         end.
