theories/Tactics.v
@@ -1,0 +1,85 @@
+(* SLOT, proofs about distributed systems design
+   Copyright (C) 2019-2021  k32
+
+   This program is free software: you can redistribute it and/or modify
+   it under the terms of the GNU General Public License as published by
+   the Free Software Foundation, version 3 of the License.
+
+   This program is distributed in the hope that it will be useful,
+   but WITHOUT ANY WARRANTY; without even the implied warranty of
+   MERCHANTABILITY or FITNESS FOR A PARTICULAR PURPOSE.  See the
+   GNU General Public License for more details.
+
+   You should have received a copy of the GNU General Public License
+   along with this program.  If not, see <https://www.gnu.org/licenses/>.
+ *)
+From Coq Require Import
+     List.
+
+Import ListNotations.
+
+From SLOT Require Import
+     Foundations.
+
+Open Scope slot_scope.
+
+Ltac long_step f tac :=
+  cbn in f;
+  lazymatch type of f with
+  | ReachableByTrace _ [] _ =>
+    let s := fresh "s" in
+    let Hx := fresh "Hx" in
+    let Hy := fresh "Hy" in
+    let Hz := fresh "Hz" in
+    inversion f as [s Hx Hy Hz|];
+    subst s; clear f; clear Hy
+  | ReachableByTrace _ (_ :: _) _ =>
+    let s' := fresh "s" in
+    let te := fresh "te" in
+    let tail := fresh "tail" in
+    let Hcr := fresh "Hcr" in
+    let Htl := fresh "Htl" in
+    inversion_clear f as [|? s' ? te tail Hcr Htl];
+    rename Htl into f;
+    cbn in Hcr;
+    tac Hcr
+  end.
+
+Tactic Notation "long_step" ident(f) tactic3(tac) := long_step f tac.
+Tactic Notation "long_step" ident(f) := long_step f (fun _ => idtac).
+
+Ltac unfold_trace f tac :=
+  repeat (long_step f tac).
+
+Tactic Notation "unfold_trace" ident(f) tactic3(tac) := unfold_trace f tac.
+Tactic Notation "unfold_trace" ident(f) := unfold_trace f (fun _ => idtac).
+Tactic Notation "unfold_trace_deep" ident(f) := unfold_trace f (fun x => inversion x); subst.
+
+Ltac ls_advance tac :=
+  match goal with
+  | [H : ReachableByTrace ?s ?t ?s' |- ?Q ?s'] =>
+    long_step H tac
+  end.
+
+Tactic Notation "ls_advance" tactic3(tac) := ls_advance tac.
+Tactic Notation "ls_advance" := ls_advance (fun _ => idtac).
+
+Hint Transparent Ensembles.In Ensembles.Complement : slot.
+Hint Constructors ReachableByTrace : slot.
+(* Hint Resolve trace_elems_commute_symm : slot. *)
+
+Ltac unfold_ht :=
+  match goal with
+  | [ |- {{?pre}} ?t {{?post}}] =>
+    let s := fresh "s_begin" in
+    let s' := fresh "s_end" in
+    let Hls := fresh "Hls" in
+    let Hpre := fresh "Hpre" in
+    intros s s' Hls Hpre;
+    match eval cbn in Hpre with
+    | [fun _ => True] => clear Hpre (* TODO: Fixme *)
+    | _ => idtac
+    end
+  | _ =>
+    fail "Goal does not look like a Hoare triple"
+  end.
